coq/bounded.v
@@ -7,32 +7,34 @@ Unset Printing Implicit Defensive.
 (** *** A fixpoint operator for bounded recursion *)
 
 Section Bounded.
-  Variables (aT rT : Type) (x0 : rT).
+  Variables (aT rT : Type) (P : aT -> Prop) (x0 : rT).
   Variables (measure : aT -> nat) (F : (aT -> rT) -> (aT -> rT)).
   
   Hypothesis F_wf : 
-    forall f g x, (forall y, measure y < measure x -> f y = g y) -> F f x = F g x.
+    forall f g x, P x -> (forall y, P y -> measure y < measure x -> f y = g y) -> F f x = F g x.
 
-  (** Note: The use of equality here effectively limits this to functions in one argument *)
+  (** Note: The use of equality here effectively limits this to
+  functions in one argument *)
   Fixpoint F_rec (n : nat) (x : aT) :=
     if n is n'.+1 then F (F_rec n') x else x0.
 
   Lemma F_rec_narrow m n x : 
-    measure x < n -> n <= m -> F_rec m x = F_rec n x.
+    P x -> measure x < n -> n <= m -> F_rec m x = F_rec n x.
   Proof.
-    elim: n m x => // => n IHn [//|m] x A B /=. 
-    apply: F_wf => y Hy. apply: IHn => //. exact: leq_trans Hy _. 
+    elim: n m x => // => n IHn [//|m] x Px A B /=. 
+    apply: F_wf => // y Py Hy. apply: IHn => //. exact: leq_trans Hy _. 
   Qed.
 
   Definition Fix x := F_rec (measure x).+1 x.
   
-  Lemma Fix_eq x : Fix x = F Fix x.
+  Lemma Fix_eq x : P x -> Fix x = F Fix x.
   Proof. 
-    rewrite /Fix /=. apply: F_wf => y Hy.
+    rewrite /Fix /= => Px. apply: F_wf => // y Py Hy.
     by rewrite (@F_rec_narrow (measure x) (measure y).+1).
   Qed.
 
 End Bounded.
+Arguments Fix_eq [aT rT] P.
 
 (** Example Instances *)
 
@@ -42,7 +44,7 @@ Definition const0 := Fix 1 id const0_rec.
 
 Lemma const0_eq n : const0 n = if n == 0 then 0 else const0 (n.-1).
 Proof. 
-  apply: Fix_eq => {n} f g n. 
+  apply: (Fix_eq xpredT) => // {n} f g n _. 
   rewrite /const0_rec. case: ifP => // /negbT. 
   case: n => //= n _ Hfg. exact: Hfg.
 Qed.
@@ -61,7 +63,7 @@ Definition foo := Fix 0 id foo_rec.
 
 Lemma foo_eq n : foo n = if n < 4 then n else \max_(m <- split n) foo m.
 Proof.
-  apply: Fix_eq => {n} g f n H.
+  apply: (Fix_eq xpredT) => // {n} g f n _ H.
   rewrite /foo_rec. case: ifP => // _. 
   apply: eq_big_seq => m /split_lt. exact: H.
 Qed.
